TWO-POINTER APPROACH

we take two pointers: 
i-> at the 0th index of the array
j-> at the last index
one approaches towards the other

for example:
index:  0  1  2  3  4   5
array = 2, 5, 7, 9, 11, 15
        i               j
target = 14

we start with calculating the sum of arr[i] and arr[j]
here, denoting the sum as 's'
so, 
    sij = arr[i] + arr[j]

s05 = 2 + 15 = 17 > target, so, we decrement j
now, 
s04 = 2 + 11 = 13 < target, so, we increment i
now,
s14 = 5 + 9 = 14 = target

therefore ans = {5, 9}